@prefix daq:     <http://purl.org/eis/vocab/daq#> .
@prefix dqm-prob:     <http://www.diachron-fp7.eu/dqm-prob#> .
@prefix owl:	 <http://www.w3.org/2002/07/owl#> .
@prefix rdf:     <http://www.w3.org/1999/02/22-rdf-syntax-ns#> .
@prefix rdfg:	 <http://www.w3.org/2004/03/trix/rdfg-1> .
@prefix rdfs:    <http://www.w3.org/2000/01/rdf-schema#> .
@prefix xsd:     <http://www.w3.org/2001/XMLSchema#> .
@prefix qpro:     <http://purl.org/eis/vocab/qpro#> .
@prefix prov: <http://www.w3.org/ns/prov#> .


### Dereferenceability
dqm-prob:SC200OK
	a	rdfs:Class;
	rdfs:subClassOf qpro:Exception ;
	rdfs:comment "The described resource has a dereferenceability Status Code of 200 instead of the required Status Code 303" ;
	rdfs:label "200 OK Status Code" .

dqm-prob:SC303WithoutParsableContent
	a	rdfs:Class;
	rdfs:subClassOf qpro:Exception ;
	rdfs:comment "The described resource has a dereferenceability Status Code of 303 but the content is not parsable due to incorrect content-type" ;
	rdfs:label "303 See Other without parsable content" .

dqm-prob:SC301MovedPermanently
	a	rdfs:Class;
	rdfs:subClassOf qpro:Exception ;
	rdfs:comment "The described resource has a dereferenceability Status Code of 301 Moved Permanently " ;
	rdfs:label "301 Moved Permanently" .

dqm-prob:SC302Found
	a	rdfs:Class;
	rdfs:subClassOf qpro:Exception ;
	rdfs:comment "The described resource has a dereferenceability Status Code of 302 Found" ;
	rdfs:label "302 Found" .

dqm-prob:SC307TemporaryRedirectory
	a	rdfs:Class;
	rdfs:subClassOf qpro:Exception ;
	rdfs:comment "The described resource has a dereferenceability Status Code of 307 Temporary Redirected" ;
	rdfs:label "307 Temporary Redirected" .

dqm-prob:SC3XXRedirection
	a	rdfs:Class;
	rdfs:subClassOf qpro:Exception ;
	rdfs:comment "The described resource has a dereferenceability Status Code of a 3XX Redirection but not the recommended 303 See Other" ;
	rdfs:label "3XX Redirection" .


dqm-prob:SC4XXClientError
	a	rdfs:Class;
	rdfs:subClassOf qpro:Exception ;
	rdfs:comment "The described resource has a dereferenceability Status Code of 4XX Client Error" ;
	rdfs:label "4XX Client Error" .


dqm-prob:SC5XXServerError
	a	rdfs:Class;
	rdfs:subClassOf qpro:Exception ;
	rdfs:comment "The described resource has a dereferenceability Status Code of 5XX Server Error" ;
	rdfs:label "5XX Server Error" .

dqm-prob:NotMeaningful
	a	rdfs:Class;
	rdfs:subClassOf qpro:Exception ;
	rdfs:comment "The described resource has a dereferenceable code as recommended by the LOD Principles (i.e. 303 See Other or Hash URI), but no meaningful data" ;
	rdfs:label "No Meaningful Data Returned" .

### RDF Accessibility

dqm-prob:NoRDFAccessibility
	a	rdfs:Class;
	rdfs:subClassOf qpro:Exception ;
	rdfs:comment "The dataset has no valid RDF Dump defined with the void:dataDump predicate" ;
	rdfs:label "RDF Dump Availablility" .

dqm-prob:InvalidDataDumpURI
	a	rdfs:Class;
	rdfs:subClassOf qpro:Exception ;
	rdfs:comment "The described URI is not a valid RDF data dump" ;
	rdfs:label "Invalid RDF Dump" .


### SPARQL EndPoint Accessibility
dqm-prob:NoEndPointAccessibility
	a	rdfs:Class;
	rdfs:subClassOf qpro:Exception ;
	rdfs:comment "The dataset has no valid SPARQL Endpoints defined with the void:sparqlEndpoint predicate" ;
	rdfs:label "SPARQL EndPoint Availablility" .

dqm-prob:InvalidSPARQLEndPoint
	a	rdfs:Class;
	rdfs:subClassOf qpro:Exception ;
	rdfs:comment "The described SPARQL endpoint is either invalid or not responding" ;
	rdfs:label "RDF Dump Availablility" .

### Misreported Content Type
dqm-prob:MisreportedTypeException
	a	rdfs:Class ;
	rdfs:subClassOf qpro:Exception ;
	rdfs:comment "The described Resource has a misreported content type";
	rdfs:label "Misreported Content Type" .

dqm-prob:expectedContentType
	a	rdf:Property ;
	rdfs:subPropertyOf qpro:extraExceptionProperty ;
	rdfs:domain	rdfs:Resource ;
	rdfs:range	rdfs:Resource .

dqm-prob:actualContentType
	a	rdf:Property ;
	rdfs:subPropertyOf qpro:extraExceptionProperty ;
	rdfs:domain	rdfs:Resource ;
	rdfs:range	rdfs:Resource .

### Dereferenced Forward Links
dqm-prob:NotValidForwardLink
	a	rdfs:Class ;
	rdfs:subClassOf qpro:Exception ;
	rdfs:comment "The described resource do not resolve in a valid Dereferenced Forward-Link" ;
	rdfs:label "Not Valid Deferenceable Forward-Link" .

dqm-prob:ViolatingTriple
	a	rdfs:Class ;
	rdfs:subClassOf qpro:Exception ;
	rdfs:comment "The described resource has a violating forward link dereferencable triple" ;
	rdfs:label "Violating Triple" .

dqm-prob:hasViolatingTriple
	a rdf:Property ;
	rdfs:subPropertyOf qpro:extraExceptionProperty ;
	rdfs:domain	rdfs:Resource ;
	rdfs:range	rdfs:Resource .


### Machine Readable Licence

dqm-prob:NoValidLicenceInDataset
	a	rdfs:Class ;
	rdfs:subClassOf qpro:Exception ;
	rdfs:comment "The described RDF Document/Dataset has no valid licence in the voID description or in its metadata" ;
	rdfs:label "No valid machine-readable licence" .


dqm-prob:NotRecommendedLicenceInDataset
	a	rdfs:Class ;
	rdfs:subClassOf qpro:Exception ;
	rdfs:comment "The described RDF Document/Dataset has a valid licence that is not recommended according to the voID W3C Standards" ;
	rdfs:label "Not Recommended machine-readable licence" .

### Machine Readable Licence

dqm-prob:NoValidLicenceInDatasetForHumans
	a	rdfs:Class ;
	rdfs:subClassOf qpro:Exception ;
	rdfs:comment "The described RDF Document/Dataset has no valid licence in the in its descriptive metadata" ;
	rdfs:label "No valid human-readable licence" .


dqm-prob:NotMachineReadableLicence
	a	rdfs:Class ;
	rdfs:subClassOf qpro:Exception ;
	rdfs:comment "The described license is not in a machine-readable format" ;
	rdfs:label "Licence is not machine-readable." .
	
## Correct URI Usage

dqm-prob:IncorrectCoolURIUsage
	a	rdfs:Class ;
	rdfs:subClassOf qpro:Exception ;
	rdfs:comment "An Incorrect URI style used for dataset. For datasets with more than 500K triples Slash URIs are suggested, whilst for less than 500K triples Hash URIs should be used" ;
	rdfs:label "Incorrect Usage of URIs" .


### Dereferenced Back Links
dqm-prob:NotValidDereferenceableBackLink
	a	rdfs:Class ;
	rdfs:subClassOf qpro:Exception ;
	rdfs:comment "The described resource do not resolve in a valid Dereferenced Link" ;
	rdfs:label "Not Valid Deferenceable Backlink" .

dqm-prob:NoBackLink
	a	rdfs:Class ;
	rdfs:subClassOf qpro:Exception ;
	rdfs:comment "The described resource does not provide a valid back link" ;
	rdfs:label "No Backlink" .

dqm-prob:hasNoBackLink
	a rdf:Property ;
	rdfs:subPropertyOf qpro:extraExceptionProperty ;
	rdfs:domain	rdfs:Resource ;
	rdfs:range	rdfs:Resource .


### Links To External Data Providers

dqm-prob:NoValidRDFDataForExternalLink
	a	rdfs:Class ;
	rdfs:subClassOf qpro:Exception ;
	rdfs:comment "The External Link provided does not give valid RDF" ;
	rdfs:label "No valid RDF for External Link" .

dqm-prob:LowPercentageOfValidPLDResources
	a	rdfs:Class ;
	rdfs:subClassOf qpro:Exception ;
	rdfs:comment "The External Link provide a low number of resources that provide RDF" ;
	rdfs:label "Low Percentage of valid RDF resources in PLD" .


### Short URIs

dqm-prob:ParametarisedURI
	a	rdfs:Class ;
	rdfs:subClassOf qpro:Exception ;
	rdfs:comment "The resource URI includes a parameterised string." ;
	rdfs:label "Parametarised URI" .

dqm-prob:LongURI
	a	rdfs:Class ;
	rdfs:subClassOf qpro:Exception ;
	rdfs:comment "According to W3C URI standards, a URI should not be longer than 80 characters including the schema. Long URIs are not recommended. Refer to CoolURIs (http://www.linkeddata.org/how-to-publish)" ;
	rdfs:label "Long URI Exception" .


### No Prolix RDF
dqm-prob:UsageOfReification
	a	rdfs:Class ;
	rdfs:subClassOf qpro:Exception ;
	rdfs:comment "The resource is using RDF reification feature (type - rdf:Statement). The use of rdf:Statement or any other prolix feature is strongly discouraged." ;
	rdfs:label "Usage of Reification in Dataset" .

dqm-prob:UsageOfContainers
	a	rdfs:Class ;
	rdfs:subClassOf qpro:Exception ;
	rdfs:comment "The resource is using RDF containers feature (type - rdf:Container). The use of rdf:Container or any other prolix feature is strongly discouraged." ;
	rdfs:label "Usage of Containers in Dataset" .


dqm-prob:UsageOfCollections
	a	rdfs:Class ;
	rdfs:subClassOf qpro:Exception ;
	rdfs:comment "The resource is using RDF collections feature. The use of rdf:Alt, rdf:Bag, rdf:List, or any other prolix feature is strongly discouraged." ;
	rdfs:label "Usage of Collections" .


### DifferentSerialisationsMetric
dqm-prob:NoMultipleFormatDefined
	a	rdfs:Class ;
	rdfs:subClassOf qpro:Exception ;
	rdfs:comment "The dataset must have more than one serialisation format defined using the void:feature predicate." ;
	rdfs:label "No format defined for a dataset" .

dqm-prob:IncorrectFormatDefined
	a	rdfs:Class ;
	rdfs:subClassOf qpro:Exception ;
	rdfs:comment "The defined format using the void:feature predicate is unknown. Check http://www.w3.org/ns/formats/." ;
	rdfs:label "Incorrect defined format/feature" .

### Undefined Classes and Properties

dqm-prob:UndefinedClass
	a	rdfs:Class ;
	rdfs:subClassOf qpro:Exception ;
	rdfs:comment "The class used is undefined in the respective schema" ;
	rdfs:label "Undefined Class" .

dqm-prob:UndefinedProperty
	a	rdfs:Class ;
	rdfs:subClassOf qpro:Exception ;
	rdfs:comment "The property used is undefined in its respective schema." ;
	rdfs:label "Undefined Property" .


### Reuse of Terms and Vocabularies

dqm-prob:UnusedSuggestedVocabulary
	a	rdfs:Class ;
	rdfs:subClassOf qpro:Exception ;
	rdfs:comment "The dataset did not use terms from the suggested vocabulary." ;
	rdfs:label "Unused suggested vocabulary" .


### Entities members of disjoint classes

dqm-prob:MultiTypedResourceWithDisjointedClasses
	a	rdfs:Class ;
	rdfs:subClassOf qpro:Exception ;
	rdfs:comment "The referred resource is multi-typed with disjoined classes." ;
	rdfs:label "Disjoined Classes Typing" .

dqm-prob:violatingDisjoinedClass
	a rdf:Property ;
	rdfs:subPropertyOf qpro:extraExceptionProperty ;
	rdfs:domain	rdfs:Resource;
	rdfs:range	rdfs:Resource .


### Entities members of disjoint classes

dqm-prob:MisplacedClass
	a	rdfs:Class ;
	rdfs:subClassOf qpro:Exception ;
	rdfs:comment "The referred resource, used a defined class instead of a property, in the property's position." ;
	rdfs:label "Misplaced Class" .

dqm-prob:hasMisplacedClass
	a rdf:Property ;
	rdfs:subPropertyOf qpro:extraExceptionProperty ;
	rdfs:domain	rdfs:Resource;
	rdfs:range	rdfs:Resource .


dqm-prob:MisplacedProperty
	a	rdfs:Class ;
	rdfs:subClassOf qpro:Exception ;
	rdfs:comment "The referred resource, used a defined property instead of a class, in an rdf:type statement object's position." ;
	rdfs:label "Misplaced Property" .

dqm-prob:hasMisplacedProperty
	a rdf:Property ;
	rdfs:subPropertyOf qpro:extraExceptionProperty ;
	rdfs:domain	rdfs:Resource;
	rdfs:range	rdfs:Resource .


### Misuse of owl:DatatypeProperty or owl:ObjectProprty
dqm-prob:MisusedDatatypeProperty
	a	rdfs:Class ;
	rdfs:subClassOf qpro:Exception ;
	rdfs:comment "The referred resource used a datatype property instead of an Object Property." ;
	rdfs:label "Misused Datatype Property" .

dqm-prob:hasMisusedDatatypeProperty
	a rdf:Property ;
	rdfs:subPropertyOf qpro:extraExceptionProperty ;
	rdfs:domain	rdfs:Resource;
	rdfs:range	rdfs:Resource .


dqm-prob:MisusedObjectProperty
	a	rdfs:Class ;
	rdfs:subClassOf qpro:Exception ;
	rdfs:comment "The referred resource used an object property instead of a datatype property." ;
	rdfs:label "Misplaced Property" .

dqm-prob:hasMisusedObjectProperty
	a rdf:Property ;
	rdfs:subPropertyOf qpro:extraExceptionProperty ;
	rdfs:domain	rdfs:Resource;
	rdfs:range	rdfs:Resource .


### CurrencyOfDataset
dqm-prob:MissingMetadataForCurrency
	a	rdfs:Class ;
	rdfs:subClassOf qpro:Exception ;
	rdfs:comment "The referred dataset have missing metadata properties thus cannot calculate currency." ;
	rdfs:label "Missing Metadata for Currency Calculation" .

dqm-prob:MissingMetadataForFreshness
	a	rdfs:Class ;
	rdfs:subClassOf qpro:Exception ;
	rdfs:comment "The referred dataset have missing metadata properties thus cannot calculate data freshness." ;
	rdfs:label "Missing Metadata for Freshness Calculation" .

dqm-prob:MissingMetadataForTimelinessOfResource
	a	rdfs:Class ;
	rdfs:subClassOf qpro:Exception ;
	rdfs:comment "The referred dataset have missing metadata properties thus cannot calculate data timeliness." ;
	rdfs:label "Missing Metadata for  Calculation" .

### Extensional Conciseness
dqm-prob:ResourceReplica
	a	rdfs:Class ;
	rdfs:subClassOf qpro:Exception ;
	rdfs:comment "The referred resource has a replica resource with a different id." ;
	rdfs:label "Resource Replica" .

### Deprecated Classes and Properties
dqm-prob:DeprecatedClass
	a	rdfs:Class ;
	rdfs:subClassOf qpro:Exception ;
	rdfs:comment "The class used is deprecated in the respective schema" ;
	rdfs:label "Deprecated Class" .

dqm-prob:DeprecatedProperty
	a	rdfs:Class ;
	rdfs:subClassOf qpro:Exception ;
	rdfs:comment "The property used is deprecated in its respective schema." ;
	rdfs:label "Deprecated Property" .

### Ontology Hijacking

dqm-prob:OntologyHijackingException
	a	rdfs:Class ;
	rdfs:subClassOf qpro:Exception ;
	rdfs:comment "The referred resource hijacked an external authorative concept." ;
	rdfs:label "Misplaced Property" .

dqm-prob:hijackedTripleStatement
	a rdf:Property ;
	rdfs:subPropertyOf qpro:extraExceptionProperty ;
	rdfs:domain	dqm-prob:OntologyHijackingException;
	rdfs:range	rdf:Statement .

dqm-prob:hijackedConcept
	a rdf:Property ;
	rdfs:subPropertyOf qpro:extraExceptionProperty ;
	rdfs:domain	dqm-prob:OntologyHijackingException ;
	rdfs:comment "Describes what concept was hijacked" ;
	rdfs:range	rdf:Statement .

dqm-prob:hijackedBy
	a rdf:Property ;
	rdfs:subPropertyOf qpro:extraExceptionProperty ;
	rdfs:domain	dqm-prob:OntologyHijackingException ;
	rdfs:comment "Describes what resource in the local dataset hijacked a property" ;
	rdfs:range	rdf:Statement .

dqm-prob:hijackedRule
	a rdf:Property ;
	rdfs:subPropertyOf qpro:extraExceptionProperty ;
	rdfs:domain	dqm-prob:OntologyHijackingException ;
	rdfs:comment "Describes what hijacking rule was detected" ;
	rdfs:range	rdf:Statement .

### IncorrectDomainOrRange
dqm-prob:IncorrectRange
	a	rdfs:Class ;
	rdfs:subClassOf qpro:Exception ;
	rdfs:comment "The property's value has an incorrect data type" ;
	rdfs:label "Undefined Class" .

dqm-prob:IncorrectDomain
	a	rdfs:Class ;
	rdfs:subClassOf qpro:Exception ;
	rdfs:comment "The property should not be used within a resource of this type." ;
	rdfs:label "Undefined Property" .

dqm-prob:UnknownType
	a	rdfs:Class ;
	rdfs:subClassOf qpro:Exception ;
	rdfs:comment "The resource type is unknown." ;
	rdfs:label "Undefined Property" .

dqm-prob:problematicTriple
	a rdf:Property ;
	rdfs:subPropertyOf qpro:extraExceptionProperty ;
	rdfs:domain	qpro:Exception;
	rdfs:range	rdf:Statement .

### IFP metric
dqm-prob:InverseFunctionalPropertyViolation
	a	rdfs:Class ;
	rdfs:subClassOf qpro:Exception ;
	rdfs:comment "The referred predicate and objects are used in multiple subject resources which violates the IFP metric." ;
	rdfs:label "Inverse Functional Property Violation" .

dqm-prob:violatedPredicate
	a rdf:Property ;
	rdfs:subPropertyOf qpro:extraExceptionProperty ;
	rdfs:domain	dqm-prob:InverseFunctionalPropertyViolation;
	rdfs:range	rdfs:Resource .

dqm-prob:violatedObject
	a rdf:Property ;
	rdfs:subPropertyOf qpro:extraExceptionProperty ;
	rdfs:domain	dqm-prob:InverseFunctionalPropertyViolation;
	rdfs:range	rdfs:Resource .

dqm-prob:violatingSubjects
	a rdf:Property ;
	rdfs:subPropertyOf qpro:extraExceptionProperty ;
	rdfs:domain	dqm-prob:InverseFunctionalPropertyViolation;
	rdfs:range	rdf:Bag .

### Understandability
dqm-prob:NoHumanReadableLabel
	a	rdfs:Class ;
	rdfs:subClassOf qpro:Exception ;
	rdfs:comment "Entities in this list have no Human Readable Label." ;
	rdfs:label "No Human Readable Label" .

dqm-prob:NoVocabularyIndication
	a	rdfs:Class ;
	rdfs:subClassOf qpro:Exception ;
	rdfs:comment "Vocabularies in this list are not indicated by a respective voID description." ;
	rdfs:label "No Vocabulary Indication" .

dqm-prob:NoURIRegExPresence
	a	rdfs:Class ;
	rdfs:subClassOf qpro:Exception ;
	rdfs:comment "No regular expression in the voID description." ;
	rdfs:label "No Regular Expression" .


### Data Cube Population Completeness

dqm-prob:MissingPopulationCoverage
	a	rdfs:Class ;
	rdfs:subClassOf qpro:Exception ;
	rdfs:comment "The referred list of objects are not covered in the dataset." ;
	rdfs:label "Missing Population Coverage" .

dqm-prob:forCodedProperty
	a rdf:Property ;
	rdfs:subPropertyOf qpro:extraExceptionProperty ;
	rdfs:domain	dqm-prob:MissingPopulationCoverage ;
	rdfs:range	rdfs:Resource .

dqm-prob:missingPopulationCoverageList
	a rdf:Property ;
	rdfs:subPropertyOf qpro:extraExceptionProperty ;
	rdfs:domain dqm-prob:MissingPopulationCoverage ;
	rdfs:range rdf:Bag .


### Correctness of Language Tag

dqm-prob:IncorrectLanguageTag
	a	rdfs:Class ;
	rdfs:subClassOf qpro:Exception ;
	rdfs:comment "The language tag assigned to a literal is incorrect." ;
	rdfs:label "Incorrect Language Tag" .

dqm-prob:actualLanguageTag
	a rdf:Property ;
	rdfs:subPropertyOf qpro:extraExceptionProperty ;
	rdfs:domain	dqm-prob:IncorrectLanguageTag ;
	rdfs:range	xsd:string .

dqm-prob:expectedLanguageTag
	a rdf:Property ;
	rdfs:subPropertyOf qpro:extraExceptionProperty ;
	rdfs:domain	dqm-prob:IncorrectLanguageTag ;
	rdfs:range	xsd:string .

dqm-prob:actualLiteralValue
	a rdf:Property ;
	rdfs:subPropertyOf qpro:extraExceptionProperty ;
	rdfs:domain	dqm-prob:IncorrectLanguageTag ;
	rdfs:range	xsd:string .
